stdlib/lampe/Stdlib/List.lean
@@ -1,0 +1,35 @@
+import «std-1.0.0-beta.12».Extracted
+import Lampe
+import Stdlib.Tp
+
+namespace Lampe.Stdlib.List
+
+open «std-1.0.0-beta.12»
+
+set_option Lampe.pp.Expr false
+set_option Lampe.pp.STHoare false
+
+/--
+Implements the ordering relation used by Noir's `Array` and `Slice` directly over Lean's `List`.
+-/
+@[reducible]
+def compareWith {α : Type}
+    (f : α → α → Ordering)
+    (self other : List α)
+  : Ordering := match self, other with
+| [], [] => .eq
+| [], _ => .lt
+| _, [] => .gt
+| x::xs, y::ys => f x y |>.then $ compareWith f xs ys
+
+@[simp]
+theorem compareWith_nil {comparator : α → α → Ordering}
+  : compareWith comparator [] [] = .eq := by
+  simp [compareWith]
+
+theorem compareWith_take_then_drop {α : Type} {a b : List α}
+    (i : ℕ)
+    (f : α → α → Ordering)
+  : compareWith f a b = (compareWith f (a.take i) (b.take i)).then (compareWith f (a.drop i) (b.drop i)) := by
+  sorry
+
