stdlib/lampe/Stdlib/Stdlib.lean
@@ -16,12 +16,15 @@ import Stdlib.Field.Mod
 import Stdlib.Hash.Mod
 import Stdlib.Hash.Poseidon2
 import Stdlib.Lib
+import Stdlib.List
 import Stdlib.Ops.Arith
 import Stdlib.Ops.Bit
 import Stdlib.Option
 import Stdlib.Panic
 import Stdlib.Slice
 import Stdlib.String
+import Stdlib.Tp
+import Stdlib.Tuple
 
 import «std-1.0.0-beta.12».Extracted
 
