stdlib/lampe/Stdlib/Tp.lean
@@ -1,0 +1,11 @@
+import «std-1.0.0-beta.12».Extracted
+import Lampe
+
+namespace Lampe.Stdlib.Tp
+
+open «std-1.0.0-beta.12»
+
+set_option Lampe.pp.Expr false
+set_option Lampe.pp.STHoare false
+
+abbrev comparator (p : Prime) (t : Tp) : Type := t.denote p → t.denote p → Ordering
