stdlib/lampe/std-1.0.0-beta.12.lean
@@ -1,3 +1,2 @@
 import «std-1.0.0-beta.12».Extracted
-import Stdlib.Stdlib
 
